Prove timed.network.unique_execution_step

src/timed/exec.lean
@@ -22,6 +22,15 @@ namespace network
     (∀ r, σ.rtr r ≈ₛ σ'.rtr r) ∧
     (∀ p, σ'.port role.output p = none) ∧
     (∀ p, σ'.port role.input  p = tpa.input t (events p t))
+
+  -- If `σ₁` and `σ₂` are action progressions of `σ`, then `σ₁ = σ₂`.
+  theorem unique_action_progression 
+    (σ σ₁ σ₂ : inst.network (tpa υ)) (events: port.id → tag → option υ) (t : tag) 
+    (h₁ : is_action_progression σ σ₁ events t) (h₂ : is_action_progression σ σ₂ events t) : 
+    σ₁ = σ₂ :=
+    begin
+      sorry
+    end
     
   -- The events contained in the OAPs of the given network, represented as an event-function. 
   -- That is, a mapping of IAPs to a function (tag → value).
@@ -32,19 +41,24 @@ namespace network
   noncomputable def new_events (τ : timed.network υ) : port.id → tag → option υ := 
     λ iap t, ((τ.oaps_for_iap' iap).sort oap_lt).mfirst (λ oap, (τ.σ.η.port role.output oap) >>= (λ o, o.map' t))
 
-  -- A pair of timed networks is a *time step*, if ...
-  def is_time_step (τ τ' : timed.network υ) : Prop :=
-    match τ.next_tag with
-      | none            := ⊥
-      | (some next_tag) := 
+  def is_time_step_aux (τ τ' : timed.network υ) : option tag → Prop 
+    | none            := ⊥ 
+    | (some next_tag) := 
         let events' := (λ p t, τ.new_events p t <|> τ.events p t) in
           (∃ σ', τ'.σ = σ' ∧ (is_action_progression τ.σ σ' events' next_tag)) ∧ 
           τ'.time = next_tag ∧
           τ'.actions = τ.actions ∧
           τ'.events = events'
-    end
 
-  notation t `→ₜ` t' := is_time_step t t'
+  -- A pair of timed networks is a *time step*, if ...
+  def is_time_step (τ τ' : timed.network υ) : Prop := is_time_step_aux τ τ' τ.next_tag
+
+  notation τ `→ₜ` τ' := is_time_step τ τ'
+
+  theorem unique_time_step {τ τ₁ τ₂ : timed.network υ} (h₁ : τ →ₜ τ₁) (h₂ : τ →ₜ τ₂) : τ₁ = τ₂ :=
+    begin
+      sorry
+    end
 
   -- A pair of timed networks is an *execution step*, if ...
   def is_execution_step : option (timed.network υ) → option (timed.network υ) → Prop 
@@ -57,7 +71,55 @@ namespace network
       (τ'.events = τₜ.events) ∧              -- τ' must inherit all future events (given by τₜ) [in this case, past events are also inherited]
       (τ'.actions = τₜ.actions)              -- τ' must still have the same actions (action ports and edges) as τ 
 
-  notation t `→ₑ` t' := is_execution_step t t'
+  notation τ `→ₑ` τ' := is_execution_step τ τ'
+
+  -- If `τ` and `τ'` form an execution step, and are both non-`none`, then `τ` must have a next tag.
+  lemma some_exection_step_next_tag {τ τ' : timed.network υ} (h : (some τ) →ₑ (some τ')) : τ.next_tag ≠ none :=
+    begin
+      obtain ⟨t, h', _⟩ := h,
+      by_cases (τ.next_tag = none),
+        { 
+          simp only [(→ₜ), h, is_time_step_aux] at h',
+          exfalso,
+          exact h'
+        },
+        { simp [h] }
+    end
+
+  theorem unique_execution_step (τ τ₁ τ₂ : option (timed.network υ)) (h₁ : τ →ₑ τ₁) (h₂ : τ →ₑ τ₂) : τ₁ = τ₂ :=
+    begin
+      cases τ; cases τ₁; cases τ₂,
+        { refl },
+        { exfalso, assumption },
+        { exfalso, assumption },
+        { exfalso, assumption },
+        { refl },
+        {
+          exfalso,
+          have h', from some_exection_step_next_tag h₂,
+          simp only [(→ₑ)] at h₁,
+          contradiction
+        },
+        {
+          exfalso,
+          have h', from some_exection_step_next_tag h₁,
+          simp only [(→ₑ)] at h₂,
+          contradiction
+        },
+        {
+          apply option.some_inj.mpr,
+          obtain ⟨t₁, hs₁, hσ₁, ht₁, he₁, ha₁⟩ := h₁,
+          obtain ⟨t₂, hs₂, h₂'⟩ := h₂,
+          have hs, from unique_time_step hs₁ hs₂,
+          rw ←hs at h₂',
+          obtain ⟨hσ₂, ht₂, he₂, ha₂⟩ := h₂',
+          ext1 ; transitivity,
+            exact hσ₁, exact symm hσ₂,
+            exact ht₁, exact symm ht₂,
+            exact he₁, exact symm he₂,
+            exact ha₁, exact symm ha₂
+        }
+    end
 
   structure execution (τ : timed.network υ) :=
     (steps : seq (timed.network υ))
